theories/rust_typing/maybe_uninit.v
@@ -45,6 +45,9 @@ Section type.
     iIntros (rt T π r v) "_". done.
   Qed.
   Next Obligation.
+    iIntros (rt T ? π r v) "_". done.
+  Qed.
+  Next Obligation.
     iIntros (rt T κ π l r) "Hl". destruct r as [r | ].
     - iDestruct "Hl" as "(%r'' & Hrfn & Hl)". iApply (ty_shr_aligned with "Hl").
     - iApply (ty_shr_aligned with "Hl").
